
PART 4:

There is no optimal strategy. No strategy effects the chances of a team to win the competition.

Let 
ğ´
=
âˆ‘
ğ‘–
=
1
ğ‘š
ğ‘
ğ‘–
A= 
i=1
âˆ‘
m
â€‹
 a 
i
â€‹
  and 
ğµ
=
âˆ‘
ğ‘–
=
1
ğ‘›
ğ‘
ğ‘–
.
B= 
i=1
âˆ‘
n
â€‹
 b 
i
â€‹
 . Then the chances of a team to win are proportional to its total strength, i.e., for the first team, it is 
ğ´
ğ´
+
ğµ
;
A+B
A
â€‹
 ; for the second, it is 
ğµ
ğ´
+
ğµ
.
A+B
B
â€‹
 .

The proof is by induction on 
ğ‘›
+
ğ‘š
,
n+m, assuming both 
ğ‘›
n and 
ğ‘š
m are greater than zero.

The claim is certainly true for 
ğ‘š
=
ğ‘›
=
1.
m=n=1. Assume it is true for 
ğ‘š
+
ğ‘›
=
ğ‘
,
m+n=N, and let now that one team still has 
ğ‘š
m members, the other membership of the other grew to 
ğ‘›
+
1.
n+1.

So now 
ğ´
=
âˆ‘
ğ‘–
=
1
ğ‘š
ğ‘
ğ‘–
A= 
i=1
âˆ‘
m
â€‹
 a 
i
â€‹
  and 
ğµ
=
âˆ‘
ğ‘–
=
1
ğ‘›
+
1
ğ‘
ğ‘–
.
B= 
i=1
âˆ‘
n+1
â€‹
 b 
i
â€‹
 .

For the first duel, the first team sends a gladiator of strength 
ğ‘
,
a, the second a gladiator of strength 
ğ‘
.
b. The first wins with the probability of 
ğ‘
ğ‘
+
ğ‘
,
a+b
a
â€‹
 , the second with the probability of 
ğ‘
ğ‘
+
ğ‘
.
a+b
b
â€‹
 .

Depending on who wins that duel, there will be two possible distributions of strength:

ğ‘
a wins: 
{
ğ‘
1
,
â€¦
,
ğ‘
+
ğ‘
,
â€¦
,
ğ‘
ğ‘š
}
{a 
1
â€‹
 ,â€¦,a+b,â€¦,a 
m
â€‹
 } and 
{
ğ‘
1
,
â€¦
,
ğ‘
â€¾
â€¦
,
ğ‘
ğ‘›
+
1
}
,
{b 
1
â€‹
 ,â€¦, 
b
 â€¦,b 
n+1
â€‹
 },

ğ‘
b wins: 
{
ğ‘
1
,
â€¦
,
ğ‘
â€¾
,
â€¦
,
ğ‘
ğ‘š
}
{a 
1
â€‹
 ,â€¦, 
a
 ,â€¦,a 
m
â€‹
 } and 
{
ğ‘
1
,
â€¦
,
ğ‘
+
ğ‘
â€¦
,
ğ‘
ğ‘›
+
1
}
,
{b 
1
â€‹
 ,â€¦,b+aâ€¦,b 
n+1
â€‹
 },

where overline means the absence of the fighter.

According to the induction assumption, in the first case, the chances of the first team to win equal 
ğ´
+
ğ‘
ğ´
+
ğµ
,
A+B
A+b
â€‹
 , in the second case they are equal to 
ğ´
âˆ’
ğ‘
ğ´
+
ğµ
,
A+B
Aâˆ’a
â€‹
 , making the overall probability to be

\begin{align} P_a &= \frac{a}{a+b} \cdot \frac{A+b}{A+B} + \frac{b}{a+b} \cdot \frac{A-a}{A+B}\ &= \frac{a(A+b) + b(A-a)}{(a+b)(A+B)}\ &= \frac{aA + ab + bA - ab}{(a+b)(A+B)}\ &= \frac{aA + bA}{(a+b)(A+B)}\ &= \frac{(a+b)A}{(a+b)(A+B)}\ &= \frac{A}{A+B} \end{align}

The code for part 4 is given below wherein we have selected any warrior at random for both the arrays.
